New proposal for FStar.Buffer with some abstract predicates. See examples/low-level/Chacha.fst

ulib/FStar.Buffer.fst
@@ -37,7 +37,7 @@ let as_aref #a (b:buffer a) : GTot Heap.aref = as_aref b.content
 let frameOf #a (b:buffer a) : GTot HH.rid = frameOf (content b)
 
 (* Liveness condition, necessary for any computation on the buffer *)
-let live #a (h:mem) (b:buffer a) : GTot Type0 = 
+abstract let live #a (h:mem) (b:buffer a) : GTot Type0 = 
   contains h b /\ max_length h b >= length b + idx b
 
 let getValue #a h (b:buffer a{live h b}) (i:nat{i<max_length h b}) : GTot a = Seq.index (sel h b) i
@@ -70,6 +70,24 @@ let includes #a (x:buffer a) (y:buffer a) : GTot Type0 =
 let disjoint #a #a' (x:buffer a) (y:buffer a') : GTot Type0 =
   frameOf x <> frameOf y \/ as_aref x <> as_aref y
   \/ (as_aref x = as_aref y /\ frameOf x = frameOf y /\ (idx x + length x <= idx y \/ idx y + length y <= idx x))
+
+let lemma_disjoint_refl #a #a' (x:buffer a) (y:buffer a') : Lemma
+  (requires (True))
+  (ensures (disjoint x y <==> disjoint y x))
+  [SMTPat (disjoint x y)]
+  = ()
+
+let lemma_disjoint_sub #a #a' (x:buffer a) (subx:buffer a) (y:buffer a') : Lemma
+  (requires (includes x subx /\ disjoint x y))
+  (ensures  (disjoint subx y))
+  [SMTPat (disjoint subx y); SMTPat (includes x subx)]
+  = ()
+
+let lemma_disjoint_sub' #a #a' (x:buffer a) (subx:buffer a) (y:buffer a') : Lemma
+  (requires (includes x subx /\ disjoint x y))
+  (ensures  (disjoint subx y))
+  [SMTPat (disjoint y subx); SMTPat (includes x subx)]
+  = ()
 
 (* Abstraction of buffers of any type *)
 #set-options "--__temp_no_proj SBuffer"
@@ -279,26 +297,26 @@ let modifies_trans_4_4 rid b b' b'' b''' h0 h1 h2 :
 (* TODO: complete with specialized versions of every general lemma *)
 
 (* Modifies clauses that do not change the shape of the HyperStack (h1.tip = h0.tip) *)
-let modifies_0 h0 h1 = 
+abstract let modifies_0 h0 h1 = 
   modifies_one h0.tip h0 h1 /\ modifies_buf_0 h0.tip h0 h1
 
-let modifies_1 (#a:Type) (b:buffer a) h0 h1 =
+abstract let modifies_1 (#a:Type) (b:buffer a) h0 h1 =
   let rid = frameOf b in
   modifies_one rid h0 h1 /\ modifies_buf_1 rid b h0 h1
 
-let modifies_2_1 (#a:Type) (b:buffer a) h0 h1 =
+abstract let modifies_2_1 (#a:Type) (b:buffer a) h0 h1 =
   let rid = frameOf b in
   ((rid = h0.tip /\ modifies_buf_1 rid b h0 h1 /\ modifies_one rid h0 h1)
   \/ (rid <> h0.tip /\ HH.modifies_just (Set.union (Set.singleton rid) (Set.singleton h0.tip)) h0.h h1.h  
       /\ modifies_buf_1 rid b h0 h1 /\ modifies_buf_0 h0.tip h0 h1 ))
 
-let modifies_2 (#a:Type) (#a':Type) (b:buffer a) (b':buffer a') h0 h1 =
+abstract let modifies_2 (#a:Type) (#a':Type) (b:buffer a) (b':buffer a') h0 h1 =
   let rid = frameOf b in let rid' = frameOf b' in
   ((rid = rid' /\ modifies_buf_2 rid b b' h0 h1 /\ modifies_one rid h0 h1)
   \/ (rid <> rid' /\ HH.modifies_just (Set.union (Set.singleton rid) (Set.singleton rid')) h0.h h1.h  
       /\ modifies_buf_1 rid b h0 h1 /\ modifies_buf_1 rid' b' h0 h1 ))
 
-let modifies_3 (#a:Type) (#a':Type) (#a'':Type) (b:buffer a) (b':buffer a')  (b'':buffer a'') h0 h1 =
+abstract let modifies_3 (#a:Type) (#a':Type) (#a'':Type) (b:buffer a) (b':buffer a')  (b'':buffer a'') h0 h1 =
   let rid = frameOf b in let rid' = frameOf b' in let rid'' = frameOf b'' in
   ((rid = rid' /\ rid' = rid'' /\ modifies_buf_3 rid b b' b'' h0 h1 /\ modifies_one rid h0 h1)
   \/ (rid = rid' /\ rid' <> rid'' /\ modifies_buf_2 rid b b' h0 h1 /\ modifies_buf_1 rid'' b'' h0 h1
@@ -311,7 +329,7 @@ let modifies_3 (#a:Type) (#a':Type) (#a'':Type) (b:buffer a) (b':buffer a')  (b'
       /\ HH.modifies_just (Set.union (Set.union (Set.singleton rid) (Set.singleton rid')) (Set.singleton rid'')) h0.h h1.h  
       /\ modifies_buf_1 rid b h0 h1 /\ modifies_buf_1 rid' b' h0 h1 /\ modifies_buf_1 rid'' b'' h0 h1))
 
-let modifies_3_2 (#a:Type) (#a':Type) (b:buffer a) (b':buffer a') h0 h1 =
+abstract let modifies_3_2 (#a:Type) (#a':Type) (b:buffer a) (b':buffer a') h0 h1 =
   let rid = frameOf b in let rid' = frameOf b' in
   ((rid = rid' /\ rid' = h0.tip /\ modifies_buf_2 rid b b' h0 h1 /\ modifies_one rid h0 h1)
   \/ (rid = rid' /\ rid' <> h0.tip /\ modifies_buf_2 rid b b' h0 h1 /\ modifies_buf_0 h0.tip h0 h1
@@ -324,7 +342,7 @@ let modifies_3_2 (#a:Type) (#a':Type) (b:buffer a) (b':buffer a') h0 h1 =
       /\ HH.modifies_just (Set.union (Set.union (Set.singleton rid) (Set.singleton rid')) (Set.singleton h0.tip)) h0.h h1.h  
       /\ modifies_buf_1 rid b h0 h1 /\ modifies_buf_1 rid' b' h0 h1 /\ modifies_buf_0 h0.tip h0 h1))
 
-let modifies_region rid bufs h0 h1 =
+abstract let modifies_region rid bufs h0 h1 =
   modifies_one rid h0 h1 /\ modifies_buf rid bufs h0 h1
 
 let lemma_stl_1 (#a:Type) (b:buffer a) h0 h1 h2 h3 : Lemma
@@ -426,7 +444,7 @@ let lemma_modifies_0_1 (#a:Type) (b:buffer a) h0 h1 h2 : Lemma
 let lemma_modifies_0_1' (#a:Type) (b:buffer a) h0 h1 h2 : Lemma
   (requires (~(contains h0 b) /\ modifies_0 h0 h1 /\ live h1 b /\ modifies_1 b h1 h2))
   (ensures  (modifies_0 h0 h2))
-  [SMTPat (modifies_0 h0 h1); SMTPat (modifies_1 b h1 h2)]
+  (* [SMTPat (modifies_0 h0 h1); SMTPat (modifies_1 b h1 h2)] *)
   = ()
 
 #reset-options "--z3timeout 100"
@@ -442,14 +460,14 @@ let lemma_modifies_0_2 (#t:Type) (#t':Type) (b:buffer t) (b':buffer t') h0 h1 h2
   (requires (live h0 b /\ ~(contains h0 b') /\ modifies_0 h0 h1 /\ live h1 b'
     /\ frameOf b' = h0.tip /\ modifies_2 b b' h1 h2))
   (ensures  (modifies_2_1 b h0 h2))
-  [SMTPat (modifies_2 b b' h1 h2); SMTPat (live h0 b)]
+  [SMTPat (modifies_2 b b' h1 h2); SMTPat (modifies_0 h0 h1)]
   = ()
 
 let lemma_modifies_0_2' (#t:Type) (#t':Type) (b:buffer t) (b':buffer t') h0 h1 h2 : Lemma
   (requires (live h0 b /\ ~(contains h0 b') /\ modifies_0 h0 h1 /\ live h1 b'
     /\ frameOf b' = h0.tip /\ modifies_2 b' b h1 h2))
   (ensures  (modifies_2_1 b h0 h2))
-  [SMTPat (modifies_2 b' b h1 h2); SMTPat (live h0 b)]
+  [SMTPat (modifies_2 b' b h1 h2); SMTPat (modifies_0 h0 h1)]
   = ()
 
 let lemma_modifies_1_2 (#t:Type) (#t':Type) (b:buffer t) (b':buffer t') h0 h1 h2 : Lemma
@@ -555,13 +573,13 @@ let upd #a b n z =
 (* Could be made Total with a couple changes in the spec *)
 let sub #a (b:buffer a) (i:UInt32.t) (len:UInt32.t{v len <= length b /\ v i + v len <= length b}) : STL (buffer a)
      (requires (fun h -> live h b))
-     (ensures (fun h0 b' h1 -> content b = content b' /\ idx b' = idx b + v i /\ length b' = v len /\ (h0 == h1 /\ includes b b')))
+     (ensures (fun h0 b' h1 -> content b = content b' /\ idx b' = idx b + v i /\ length b' = v len /\ (h0 == h1 /\ includes b b' /\ live h1 b')))
   = {content = b.content; idx = i +^ b.idx; length = len}
 
 let offset #a (b:buffer a) (i:UInt32.t{v i <= length b}) : STL (buffer a)
   (requires (fun h -> live h b))
   (ensures (fun h0 b' h1 -> content b' = content b /\ idx b' = idx b + v i /\ length b' = length b - v i
-    /\ h0 == h1 /\ includes b b'))
+    /\ h0 == h1 /\ includes b b' /\ live h1 b'))
   = {content = b.content; idx = i +^ b.idx; length = b.length -^ i}
 
 let lemma_modifies_one_trans_1 (#a:Type) (b:buffer a) (h0:mem) (h1:mem) (h2:mem): Lemma
@@ -797,8 +815,67 @@ let modifies_popped_0 h0 h1 h2 h3 : Lemma
   [SMTPat (fresh_frame h0 h1); SMTPat (popped h2 h3); SMTPat (modifies_0 h1 h2)]
   = ()
 
+let live_popped (#t:Type) (b:buffer t) h0 h1 : Lemma
+  (requires (popped h0 h1 /\ live h0 b /\ frameOf b <> h0.tip))
+  (ensures  (live h1 b))
+  [SMTPat (popped h0 h1); SMTPat (live h0 b)]
+  = ()
+
+let live_fresh (#t:Type) (b:buffer t) h0 h1 : Lemma
+  (requires (fresh_frame h0 h1 /\ live h0 b))
+  (ensures  (live h1 b))
+  [SMTPat (fresh_frame h0 h1); SMTPat (live h0 b)]
+  = ()
+
 let modifies_0_to_2_1_lemma (#t:Type) h0 h1 (b:buffer t) : Lemma
   (requires (modifies_0 h0 h1 /\ live h0 b))
   (ensures  (modifies_2_1 b h0 h1))
   [SMTPat (modifies_2_1 b h0 h1); SMTPat (live h0 b) ]
+  = ()
+
+let modifies_poppable_0 h0 h1 : Lemma
+  (requires (modifies_0 h0 h1 /\ HS.poppable h0))
+  (ensures  (HS.poppable h1))
+  [SMTPat (modifies_0 h0 h1)]
+  = ()
+
+let modifies_poppable_1 #t h0 h1 (b:buffer t) : Lemma
+  (requires (modifies_1 b h0 h1 /\ HS.poppable h0))
+  (ensures  (HS.poppable h1))
+  [SMTPat (modifies_1 b h0 h1)]
+  = ()
+
+let modifies_poppable_2_1 #t h0 h1 (b:buffer t) : Lemma
+  (requires (modifies_2_1 b h0 h1 /\ HS.poppable h0))
+  (ensures  (HS.poppable h1))
+  [SMTPat (modifies_2_1 b h0 h1)]
+  = ()
+
+let modifies_poppable_2 #t #t' h0 h1 (b:buffer t) (b':buffer t') : Lemma
+  (requires (modifies_2 b b' h0 h1 /\ HS.poppable h0))
+  (ensures  (HS.poppable h1))
+  [SMTPat (modifies_2 b' b h0 h1)]
+  = ()
+
+let modifies_poppable_3_2 #t #t' h0 h1 (b:buffer t) (b':buffer t') : Lemma
+  (requires (modifies_3_2 b b' h0 h1 /\ HS.poppable h0))
+  (ensures  (HS.poppable h1))
+  [SMTPat (modifies_3_2 b' b h0 h1)]
+  = ()
+
+let lemma_fresh_poppable h0 h1 : Lemma
+  (requires (fresh_frame h0 h1))
+  (ensures  (poppable h1))
+  [SMTPat (fresh_frame h0 h1)]
+  = ()
+
+let lemma_equal_domains_popped h0 h1 h2 h3 : Lemma
+  (requires (equal_domains h0 h1 /\ popped h0 h2 /\ popped h1 h3))
+  (ensures  (equal_domains h2 h3))  
+  = ()
+
+let lemma_equal_domains h0 h1 h2 h3 h4 : Lemma
+  (requires (fresh_frame h0 h1 /\ modifies_0 h1 h2 /\ equal_domains h2 h3 /\ popped h3 h4))
+  (ensures  (equal_domains h0 h4))
+  [SMTPat (fresh_frame h0 h1); SMTPat (modifies_0 h1 h2); SMTPat (popped h3 h4)]
   = ()
